probability/probabilistic_relations/Examples/utp_prob_rel_lattice_parallel_examples.thy
@@ -1,0 +1,115 @@
+section \<open> Example of probabilistic relation programming: parallel composition \<close>
+
+theory utp_prob_rel_lattice_parallel_examples
+  imports 
+    "../utp_prob_rel_lattice_laws" 
+begin 
+
+unbundle UTP_Syntax
+
+declare [[show_types]]
+
+alphabet state1 = 
+  b :: \<bool>
+
+lemma if_div_distrib: "(if a then (bb::\<real>) else c) / d = (if a then (bb / d) else (c /d))"
+  by presburger
+
+lemma if_div_distrib': "n * (if a then (bb::\<real>) else c) / d = (if a then (n * bb / d) else (n * c /d))"
+  by presburger
+
+text \<open>This example is from Hehner's paper "a Probability Perspective" 
+\cite[Sect.~Probabilistic programming]{Hehner2011} \<close>
+term "\<lbrakk>(b := e) :: state1 rel\<rbrakk>\<^sub>P"
+term "(b\<^sup>> = f)\<^sub>e"
+
+lemma b_assign_rel: "\<lbrakk>(b := e) :: state1 rel\<rbrakk>\<^sub>P = (b\<^sup>> = e\<^sup><)\<^sub>e"
+  apply (simp add: expr_defs)
+  by (rel_auto)
+
+lemma r1_3: "(real_of_ereal (ureal2ereal (ereal2ureal' (min ((1::ereal) / ereal (3::\<real>)) (1::ereal))))) = 1/3"
+  using ereal_1_div real2uereal_min_inverse' by auto
+
+lemma "(((if\<^sub>p 1/3 then b := False else b := True) \<parallel> (if\<^sub>p 1/3 then b := (\<not> b) else II))::state1 prhfun) = 
+  prfun_of_rvfun ((5 - 3 * \<lbrakk>b\<^sup><\<rbrakk>\<^sub>\<I>\<^sub>e + 6 * \<lbrakk>b\<^sup>< \<and> b\<^sup>>\<rbrakk>\<^sub>\<I>\<^sub>e) / 10)\<^sub>e "
+  apply (simp add: pparallel_pp_def)
+  apply (simp add: prfun_skip[where x = "b"])
+  apply (subst prfun_pchoice_assigns_inverse_c')
+  apply (subst prfun_pchoice_assigns_inverse_c')
+  apply (simp only: b_assign_rel)
+  apply (simp only: pparallel_def)
+  apply (simp add: expr_defs rel lens_defs prod.case_eq_if alpha_splits dist_defs)
+  apply (rule HOL.arg_cong[where f="prfun_of_rvfun"])
+  apply (simp add: ureal_defs r1_3)
+  apply (subst fun_eq_iff, rule allI)
+proof -
+  fix x::"state1 \<times> state1"
+  let ?sum = "(\<Sum>\<^sub>\<infinity>v\<^sub>0::state1.
+          ((if \<not> b\<^sub>v v\<^sub>0 then 1::\<real> else (0::\<real>)) / (3::\<real>) +
+           (2::\<real>) * (if b\<^sub>v v\<^sub>0 then 1::\<real> else (0::\<real>)) / (3::\<real>)) *
+          ((if b\<^sub>v v\<^sub>0 = (\<not> b\<^sub>v (fst x)) then 1::\<real> else (0::\<real>)) / (3::\<real>) +
+           (2::\<real>) * (if b\<^sub>v v\<^sub>0 = b\<^sub>v (fst x) then 1::\<real> else (0::\<real>)) / (3::\<real>)))"
+  have card_1: "(card {s::state1. \<not> b\<^sub>v s \<and> b\<^sub>v s = (\<not> b\<^sub>v (fst x))}) 
+    = (if b\<^sub>v (fst x) then 1 else 0)"
+    apply (simp)
+    by (smt (verit, ccfv_threshold) card_1_singleton state1.cases state1.select_convs(1))
+  have card_2: "(card {s::state1. \<not> b\<^sub>v s \<and> b\<^sub>v s = b\<^sub>v (fst x)}) 
+    = (if \<not>b\<^sub>v (fst x) then 1 else 0)"
+    apply (auto)
+    by (smt (verit) card_1_singleton state1.cases state1.select_convs(1) state1.update_convs(1))
+
+  have card_3: "(card {s::state1. b\<^sub>v s \<and> b\<^sub>v s = (\<not> b\<^sub>v (fst x))}) 
+    = (if \<not>b\<^sub>v (fst x) then 1 else 0)"
+    apply (auto)
+    by (smt (verit) card_1_singleton state1.cases state1.select_convs(1) state1.update_convs(1))
+
+  have card_4: "(card {s::state1. b\<^sub>v s \<and> b\<^sub>v s = b\<^sub>v (fst x)}) 
+    = (if b\<^sub>v (fst x) then 1 else 0)"
+    apply (auto)
+    by (smt (verit) card_1_singleton state1.cases state1.select_convs(1) state1.update_convs(1))
+
+  have sum_1: "?sum = (\<Sum>\<^sub>\<infinity>v\<^sub>0::state1.
+       (if \<not> b\<^sub>v v\<^sub>0 then 1::\<real> else (0::\<real>)) / (3::\<real>) *
+       ((if b\<^sub>v v\<^sub>0 = (\<not> b\<^sub>v (fst x)) then 1::\<real> else (0::\<real>)) / (3::\<real>)) +
+       (if \<not> b\<^sub>v v\<^sub>0 then 1::\<real> else (0::\<real>)) / (3::\<real>) *
+       ((2::\<real>) * (if b\<^sub>v v\<^sub>0 = b\<^sub>v (fst x) then 1::\<real> else (0::\<real>)) / (3::\<real>)) +
+       ((2::\<real>) * (if b\<^sub>v v\<^sub>0 then 1::\<real> else (0::\<real>)) / (3::\<real>) *
+        ((if b\<^sub>v v\<^sub>0 = (\<not> b\<^sub>v (fst x)) then 1::\<real> else (0::\<real>)) / (3::\<real>)) +
+        (2::\<real>) * (if b\<^sub>v v\<^sub>0 then 1::\<real> else (0::\<real>)) / (3::\<real>) *
+        ((2::\<real>) * (if b\<^sub>v v\<^sub>0 = b\<^sub>v (fst x) then 1::\<real> else (0::\<real>)) / (3::\<real>))))"
+    apply (simp only: ring_distribs(2))
+    by (simp only: ring_distribs(1))
+   also have sum_2: "... = (\<Sum>\<^sub>\<infinity>v\<^sub>0::state1.
+          (if \<not> b\<^sub>v v\<^sub>0 then 1::\<real> else (0::\<real>)) *
+             (if b\<^sub>v v\<^sub>0 = (\<not> b\<^sub>v (fst x)) then 1::\<real> else (0::\<real>)) / (9::\<real>) +
+       (if \<not> b\<^sub>v v\<^sub>0 then 1::\<real> else (0::\<real>)) *
+         (if b\<^sub>v v\<^sub>0 = b\<^sub>v (fst x) then 1::\<real> else (0::\<real>)) * ((2::\<real>) / (9::\<real>)) +
+       ((if b\<^sub>v v\<^sub>0 then 1::\<real> else (0::\<real>)) *
+         (if b\<^sub>v v\<^sub>0 = (\<not> b\<^sub>v (fst x)) then 1::\<real> else (0::\<real>)) * ((2::\<real>) / (9::\<real>))) +
+       ((if b\<^sub>v v\<^sub>0 then 1::\<real> else (0::\<real>)) *
+         (if b\<^sub>v v\<^sub>0 = b\<^sub>v (fst x) then 1::\<real> else (0::\<real>)) * (4 / (9::\<real>))))"
+    apply (rule infsum_cong)
+     by (simp)
+   also have sum_3: "... = (if b\<^sub>v (fst x) then 5 else 4) / 9"
+     apply (subst conditional_conds_conj)+
+     apply (simp only: divide_inverse)
+     apply (subst infsum_constant_finite_states_4)
+     using card_1 not_finite_existsD apply force
+     using card_2 not_finite_existsD apply force
+     using card_3 not_finite_existsD apply force
+     using card_4 not_finite_existsD apply force
+     by (simp add: card_1 card_2 card_3 card_4)
+  
+  show "((if \<not> b\<^sub>v (snd x) then 1::\<real> else (0::\<real>)) / (3::\<real>) +
+        (2::\<real>) * (if b\<^sub>v (snd x) then 1::\<real> else (0::\<real>)) / (3::\<real>)) *
+       ((if b\<^sub>v (snd x) = (\<not> b\<^sub>v (fst x)) then 1::\<real> else (0::\<real>)) / (3::\<real>) +
+        (2::\<real>) * (if b\<^sub>v (snd x) = b\<^sub>v (fst x) then 1::\<real> else (0::\<real>)) / (3::\<real>)) /
+       ?sum =
+       ((5::\<real>) - (3::\<real>) * (if b\<^sub>v (fst x) then 1::\<real> else (0::\<real>)) +
+        (6::\<real>) * (if b\<^sub>v (fst x) \<and> b\<^sub>v (snd x) then 1::\<real> else (0::\<real>))) /
+       (10::\<real>)"
+    apply (simp only: sum_1 sum_2 sum_3)
+    by (auto)
+qed
+
+end
